

Problem 1.

1. Proof By Induction

Base case ($n = 1$)

Left side: $\sum_{i=1}^1 (2i-1)^2 = (1)^2 = 1$

Right side: $1*(2*1 - 1)*(2*1 + 1) / 3 = (1*1*3)/3 = 1$

So $P(1)$ is true.

Assume $P(k)$ true for some $k \geq 1$:

$$\sum_{i=1}^k (2i - 1)^2 = k(2k - 1)(2k + 1) / 3$$

Show $P(k) \rightarrow P(k+1)$

$$\sum_{i=1}^{k+1} (2i - 1)^2$$

$$= [\sum_{i=1}^k (2i - 1)^2] + (2(k+1) - 1)^2$$

$$k(2k - 1)(2k + 1)/3 + (2k + 1)^2$$

$$\text{Simplify } (2k + 1)^2 = 4k^2 + 4k + 1 = (12k^2 + 12k + 3)/3$$

$$[k(2k - 1)(2k + 1) + 12k^2 + 12k + 3] / 3$$

$$\text{Expand } k(2k - 1)(2k + 1) = k(4k^2 - 1) = 4k^3 - k$$

The numerator becomes:

$$4k^3 - k + 12k^2 + 12k + 3$$

$$= 4k^3 + 12k^2 + 11k + 3$$

Now factor the numerator as $(k + 1)(2k + 1)(2k + 3)$:

$$(k+1)(2k+1)(2k+3)$$

$$= (k+1)(4k^2 + 8k + 3)$$

$$= 4k^3 + 8k^2 + 3k + 4k^2 + 8k + 3$$

$$= 4k^3 + 12k^2 + 11k + 3$$

$$\sum_{i=1}^{k+1} (2i - 1)^2$$

$$= (k+1)(2k+1)(2k+3) / 3$$

$$2k+1 = 2(k+1) - 1, \text{ and } 2k+3 = 2(k+1) + 1$$

$$= (k+1)(2(k+1) - 1)(2(k+1) + 1) / 3$$

$P(k+1)$ holds true.

Problem 2.

Formal Definition $M = (Q, \Sigma, \delta, q_0, F)$:

1. States (Q):

- $Q = \{q_e, q_o, q_0s, q_trap\}$
- q_e : Even number of 1s seen
- q_o : Odd number of 1s seen.
- q_0s : 0s only segment
- q_trap : Invalid string found.

2. Alphabet (Σ):

$\Sigma = \{0, 1\}$

3. Start State (q_0):

$q_0 = q_e$

4. Accept States (F):

$F = \{q_e, q_0s\}$

5. Transition Function (δ)

- From State q_e :
 - 1. - $\delta(q_e, 0) = q_0s$
 - 2. - $\delta(q_e, 1) = q_o$
- From State q_o :
 - 1. $\delta(q_o, 0) = q_o$
 - 2. $\delta(q_o, 1) = q_e$
- From State q_0s :
 - $\delta(q_0s, 0) = q_0s$
 - $\delta(q_0s, 1) = q_trap$
- From State q_trap :
 - 1. $\delta(q_trap, 0) = q_trap$
 - 2. $\delta(q_trap, 1) = q_trap$

Problem 3

States: $Q = \{q_0, q_1, q_2, q_3\}$

Start State: q_0

Accept States (F): $F = \{q_0, q_3\}$

a. String: 0001

- Path: $q_0 \rightarrow(0) q_0 \rightarrow(0) q_0 \rightarrow(0) q_0 \rightarrow(1) q_1$
- Final State: q_1
- Result: Reject

b. String: 10011

- Path: $q_0 \rightarrow(1) q_1 \rightarrow(0) q_2 \rightarrow(0) q_1 \rightarrow(1) q_3 \rightarrow(1) q_3$
- Final State: q_3
- Result: Accept

c. String: 1101

- Path: $q_0 \rightarrow(1) q_1 \rightarrow(1) q_3 \rightarrow(0) q_2 \rightarrow(1) q_0$
- Final State: q_0
- Result: Accept

d. String: 11100

- Path: $q_0 \rightarrow(1) q_1 \rightarrow(1) q_3 \rightarrow(1) q_3 \rightarrow(0) q_2 \rightarrow(0) q_1$
- Final State: q_1
- Result: Reject

Problem 4

$L1 = \{w: 100 \text{ is not a substring of } w\}$
 $L2 = \{w: 2 \leq |w| \leq 4\}$

1. DFA M1 (for L1)

1. States ($Q1$):
 $Q1 = \{s, q1, q10, q100\}$
2. Start State ($q0_1$):
 $q0_1 = s$
3. Accept States ($F1$):
 $F1 = \{s, q1, q10\}$
4. Transitions (δ_1):
 - $\delta_1(s, 0) = s$
 - $\delta_1(s, 1) = q1$
 - $\delta_1(q1, 0) = q10$
 - $\delta_1(q1, 1) = q1$
 - $\delta_1(q10, 0) = q100$ (100 seen)
 - $\delta_1(q10, 1) = q1$
 - $\delta_1(q100, 0) = q100$
 - $\delta_1(q100, 1) = q100$

2. DFA M2 (for L2)

1. States ($Q2$):
 $Q2 = \{t0, t1, t2, t3, t4\}$
2. Start State ($q0_2$):
 $q0_2 = t0$
3. Accept States ($F2$):
 $F2 = \{t2, t3, t4\}$
4. Transitions (δ_2):

- $\delta_2(t_0, 0/1) = t_1$
- $\delta_2(t_1, 0/1) = t_2$
- $\delta_2(t_2, 0/1) = t_3$
- $\delta_2(t_3, 0/1) = t_4$
- $\delta_2(t_4, 0/1) = t_4$

3. Union DFA M (for $L = L_1 \cup L_2$)

1. States (Q):

$$Q = \{(q_A, q_B) \mid q_A \text{ in } Q_1, q_B \text{ in } Q_2\}$$

2. Start State (q_0):

$$q_0 = (s, t_0)$$

3. Accept States (F):

(q_A, q_B) is accepted if q_A is in F_1 OR q_B is in F_2 .

$$F = \{(q_A, q_B) \mid q_A \text{ in } \{s, q_1, q_{10}\} \text{ OR } q_B \text{ in } \{t_2, t_3, t_4\}\}$$

4. Transitions (δ):

$$\delta((q_A, q_B), x) = (\delta_1(q_A, x), \delta_2(q_B, x))$$